examples-c/linked-lists/list.h
@@ -41,7 +41,7 @@ typedef struct struct_list {
 
 /*@ predicate length_order(Length l1, Length l2) */
 
-/*@ predicate lpath(list p1, plist l, list p2) reads p1->tl */
+/*@ predicate lpath(list p1, plist l, list p2) reads p1->tl,\block_length(p1) */
 
 /*@ axiom Path_null_ax : \forall list p; lpath(p,nil(),p) */
 
