examples-c/linked-lists/coq/reverse_spec_why.v
@@ -70,8 +70,7 @@ Admitted.
 Admitted.
 
 (*Why logic*) Definition cyclic :
-  ((memory) ((pointer) global) global) -> alloc_table
-  -> ((pointer) global) -> Prop.
+  ((memory) ((pointer) global) global) -> ((pointer) global) -> Prop.
 Admitted.
 
 (*Why logic*) Definition disjoint : plist -> plist -> Prop.
@@ -89,8 +88,7 @@ Admitted.
 Admitted.
 
 (*Why logic*) Definition finite :
-  ((memory) ((pointer) global) global) -> alloc_table
-  -> ((pointer) global) -> Prop.
+  ((memory) ((pointer) global) global) -> ((pointer) global) -> Prop.
 Admitted.
 
 (*Why predicate*) Definition llist  (tl_global:((memory) ((pointer) global)
@@ -113,9 +111,8 @@ Admitted.
 Admitted.
 
 (*Why logic*) Definition length :
-  ((memory) ((pointer) global) global) -> alloc_table
-  -> ((pointer) global) -> Length.
-exact (fun tl a p => length global a tl p). 
+  ((memory) ((pointer) global) global) -> ((pointer) global) -> Length.
+exact (fun tl p => length global tl p). 
 Defined.
 
 (*Why logic*) Definition length_order : Length -> Length -> Prop.
